protocols/PORExtended.v
@@ -56,18 +56,27 @@ From protocols Require Import
 
 Import SafetyAutomation.
 
-Definition stuck_model_step_user_stuck_user {t__hon t__adv}
+Inductive indexedStep {t__hon t__adv : type} (uid : user_id) :
+  (RealWorld.universe t__hon t__adv * IdealWorld.universe t__hon)
+  -> (RealWorld.universe t__hon t__adv * IdealWorld.universe t__hon)
+  -> Prop :=
+| RealSilent : forall ru ru' iu,
+    indexedRealStep uid Silent ru ru'
+    -> indexedStep uid (ru, iu) (ru', iu)
+| BothLoud : forall ru ru' iu iu' iu'' ra ia,
+    indexedRealStep uid (Action ra) ru ru'
+    -> (indexedIdealStep uid Silent) ^* iu iu'
+    -> indexedIdealStep uid (Action ia) iu' iu''
+    -> action_matches ru.(all_ciphers) ru.(all_keys) ra ia
+    -> indexedStep uid (ru, iu) (ru', iu'')
+.
+
+Definition not_stuck_by_labels {t__hon t__adv}
            (st : universe t__hon t__adv * IdealWorld.universe t__hon) : Prop :=
   forall uid u,
     (fst st).(users) $? uid = Some u
-    -> (forall st', model_step_user uid st st' -> False)
-    -> (forall lbl bd, step_user lbl (Some uid) (build_data_step (fst st) u) bd -> False). 
-
-
-Definition try_this {t__hon t__adv}
-           (st : universe t__hon t__adv * IdealWorld.universe t__hon) : Prop :=
-  (forall uid st', model_step_user uid st st' -> False)
-  -> (forall uid u lbl bd, (fst st).(users) $? uid = Some u -> step_user lbl (Some uid) (build_data_step (fst st) u) bd -> False). 
+    -> (forall st', indexedStep uid st st' -> False)
+    -> (forall lbl ru', indexedRealStep uid lbl (fst st) ru' -> False).
 
 Lemma user_step_label_deterministic :
   forall A B C lbl1 lbl2 bd bd1' bd2' suid,
@@ -87,6 +96,10 @@ Proof.
   invert H.
   invert H6.
 Qed.
+
+Hint Resolve
+     indexedIdealStep_ideal_step
+     indexedRealStep_real_step : core.
 
 Lemma syntactically_safe_U_preservation_step :
   forall t__hon t__adv (st st' : universe t__hon t__adv * IdealWorld.universe t__hon),
@@ -109,65 +122,32 @@ Proof.
   eapply IHtrc; eauto using syntactically_safe_U_preservation_step, goodness_preservation_step.
 Qed.
 
-(* Lemma try_this_implies_labels_align : *)
-(*   forall t__hon t__adv st, *)
-(*     @try_this t__hon t__adv st *)
-(*     -> labels_align st. *)
-(* Proof. *)
-(*   unfold try_this, labels_align; *)
-(*     destruct st as [ru iu]; intros. *)
-
-(*   invert H0. *)
-
-(*   destruct (classic (exists st, model_step_user u_id (ru,iu) st)). *)
-(*   - split_ex. *)
-(*     invert H0; *)
-(*       destruct ru, userData, userData0; *)
-(*       unfold build_data_step in *; *)
-(*       simpl in *; *)
-(*       clean_map_lookups. *)
-
-(*     + admit. *)
-(*     + destruct (x ==n u_id); subst; clean_map_lookups; eauto. *)
-(*       admit. (* easy *) *)
-      
-
-(*     + pose proof (user_step_label_deterministic _ _ _ _ _ _ _ _ _ H2 H6); discriminate. *)
-(*     + pose proof (user_step_label_deterministic _ _ _ _ _ _ _ _ _ H2 H6). *)
-(*       invert H0. *)
-(*       (do 3 eexists); repeat simple apply conj; eauto. *)
-
-(*   - assert (forall st', ~ model_step_user u_id (ru,iu) st') by eauto using all_not_not_ex. *)
-(*     eapply H in H3; eauto. *)
-(*     contradiction. *)
-(* Qed. *)
-
-
-Lemma stuck_model_step_user_stuck_user_implies_labels_align :
+Lemma not_stuck_by_labels_implies_labels_align :
   forall t__hon t__adv st,
-    @stuck_model_step_user_stuck_user t__hon t__adv st
+    @not_stuck_by_labels t__hon t__adv st
     -> labels_align st.
 Proof.
-  unfold stuck_model_step_user_stuck_user, labels_align;
+  unfold not_stuck_by_labels, labels_align;
     destruct st as [ru iu]; intros.
 
   invert H0.
   specialize (H _ _ H1).
 
-  destruct (classic (exists st, model_step_user u_id (ru,iu) st)).
+  destruct (classic (exists st, indexedStep uid (ru,iu) st)).
   - split_ex.
-    invert H0;
-      destruct ru, userData, userData0;
-      unfold build_data_step in *;
-      simpl in *;
-      clean_map_lookups.
+    repeat
+      match goal with
+      | [ H : indexedStep _ _ _ |- _ ] => invert H
+      | [ H : indexedRealStep _ _ _ _ |- _ ] => invert H
+      | [ LK1 : users ?ru $? ?uid = Some ?ud1, LK2 : users ?ru $? ?uid = Some ?ud2 |- _ ] =>
+        destruct ru, ud1, ud2; unfold build_data_step in *; simpl in *; clean_map_lookups
+      | [ S1 : step_user _ (Some ?uid) _ _ , S2 : step_user _ (Some ?uid) _ _ |- _ ] =>
+        eapply user_step_label_deterministic in S1; eauto; clean_context
+      end.
 
-    + pose proof (user_step_label_deterministic _ _ _ _ _ _ _ _ _ H2 H6); discriminate.
-    + pose proof (user_step_label_deterministic _ _ _ _ _ _ _ _ _ H2 H6).
-      invert H0.
       (do 3 eexists); repeat simple apply conj; eauto.
 
-  - assert (forall st', ~ model_step_user u_id (ru,iu) st') by eauto using all_not_not_ex.
+  - assert (forall st', ~ indexedStep uid (ru,iu) st') by eauto using all_not_not_ex.
     eapply H in H3; eauto.
     contradiction.
 Qed.
@@ -386,36 +366,6 @@ Proof.
       eauto.
 Qed.
 
-(* Lemma action_matches_addnl_key : *)
-(*   forall cs gks kid k ia t (msg : crypto t) pat froms, *)
-(*     ~ In kid gks *)
-(*     -> match msg with *)
-(*       | Content _ => False *)
-(*       | SignedCiphertext cid =>  *)
-(*     -> (forall kid' kp, findKeysCrypto cs msg $? kid' = Some kp -> gks $? kid' <> None) *)
-(*     -> action_matches cs (gks $+ (kid,k)) (Input msg pat froms) ia *)
-(*     -> action_matches cs gks (Input msg pat froms) ia. *)
-(* Proof. *)
-(*   intros * NIN FIND AM; *)
-(*     invert AM; *)
-(*     unfold findKeysCrypto in FIND; *)
-(*     context_map_rewrites. *)
-
-(*   eapply InpSig; eauto using message_content_eq_addnl_key_inv. *)
-(*   eapply InpEnc; eauto using message_content_eq_addnl_key_inv. *)
-
-
-  
-(*     destruct (kid ==n kid0); subst; *)
-(*       match goal with *)
-(*       | [ H : SignedCiphertext _ = SignedCiphertext _ |- _ ] => invert H *)
-(*       end; *)
-(*       clean_map_lookups; *)
-(*       [ econstructor 1 | econstructor 2]; *)
-(*       eauto. *)
-(* Qed. *)
-
-
 Lemma no_model_step_other_user_silent_step' :
   forall t t__hon t__adv suid lbl bd bd',
 
@@ -441,11 +391,11 @@ Lemma no_model_step_other_user_silent_step' :
       -> forall lbl' bd'', step_user lbl' (Some uid') (build_data_step (mkUniverse usrs adv cs gks) ud') bd''
       -> uid <> uid'
       -> forall cmdc ,
-        (forall st', model_step_user
+        (forall st', indexedStep
                   uid' 
                   (mkUniverse usrs adv cs gks, iu)
                   st' -> False)
-      -> (forall st', model_step_user
+      -> (forall st', indexedStep
                   uid'
                   (mkUniverse (usrs' $+ (uid, mkUserData ks' cmdc qmsgs' mycs' froms' sents' n'))
                               adv' cs' gks', iu)
@@ -454,7 +404,9 @@ Proof.
   Local Ltac solve_model_step_block stp :=
     repeat
       match goal with
-      | [ H : model_step_user _ _ _ |- _ ] => 
+      | [ H : indexedStep _ _ _ |- _ ] => 
+        invert H; unfold build_data_step in *; simpl in *; clean_map_lookups
+      | [ H : indexedRealStep _ _ _ _ |- _ ] =>
         invert H; unfold build_data_step in *; simpl in *; clean_map_lookups
       | [ H1 : step_user ?lbl (Some ?uid) (?usrs,_,_,_,_,_,_,_,_,_,_) ?bd,
           H2 : step_user ?lbl__known (Some ?uid) (?usrs $+ (_,_),_,_,_,_,_,_,_,_,_,_) _ |- _ ] => 
@@ -464,8 +416,7 @@ Proof.
             (clean_map_lookups;
              eapply (user_step_label_deterministic' _ _ _ _ _ _ _ stp);
              eauto; unfold build_data_step; simpl; eauto); subst
-        (* assert (lbl = lbl__known) by admit; subst *)
-      | [ H : (forall _, model_step_user ?uid ({| users := ?usrs |},_) _ -> False),
+      | [ H : (forall _, indexedStep ?uid ({| users := ?usrs |},_) _ -> False),
           STP : step_user ?lbl (Some ?uid) (?usrs,_,_,_,_,_,_,_,_,_,_) _
           |- False ] =>
         is_not_var lbl;
@@ -485,72 +436,86 @@ Proof.
       intros; subst; eauto; clean_context;
         solve_model_step_block STEP.
 
-  - destruct userData; simpl in *.
+  - destruct userData; simpl in *; clean_map_lookups.
     destruct ra.
+
+    Ltac process_actions :=
+      repeat
+        match goal with
+        | [ H : step_user (Action (Input _ _ _)) (Some _) _ _ |- _ ] =>
+          eapply input_action_msg_queue in H; eauto; split_ex; subst
+        | [ H : step_user (Action (Output _ _ _ _)) (Some _) _ _ |- _ ] =>
+          eapply output_action_msg_queue in H; eauto; split_ex; subst
+        | [ NA1 : nextAction ?p _ , NA2 : nextAction ?p _ |- _ ] =>
+          eapply na_deterministic in NA1; eauto; split_ex
+        | [ H : ?a = ?a |- _ ] => clear H
+        | [ NA : nextAction ?p ?n , SSU : syntactically_safe_U _ , USR : _ $? ?uid = Some ( {| protocol := ?p |} ) |- _ ] =>
+            match goal with
+            | [ H : syntactically_safe uid _ _ p _ |- _ ] =>
+              eapply syntactically_safe_na in NA; eauto; split_ex
+            | [ H : syntactically_safe uid _ _ n _ |- _ ] =>
+              idtac "how?"
+            | _ => generalize (SSU _ _ _ USR eq_refl); intros; split_ex; simpl in *
+            end
+        | [ H : ?arg = _ |- _ ] =>
+          match type of arg with
+          | user_cmd _    => invert H
+          | user_cmd_type => invert H
+          | list _        => invert H
+          end
+        | [ H : _ ~= _ |- _ ] => invert H
+        | [ TC : typingcontext_sound _ ?usrs _ ?uid , SS : syntactically_safe ?uid _ _ (Recv ?p) _ |- _ ] =>
+          prop_not_exists (msg_pattern_safe (findUserKeys usrs) p);
+          assert (msg_pattern_safe (findUserKeys usrs) p) by
+              (unfold typingcontext_sound in TC; split_ex; invert SS; process_ctx; eauto)
+        | [ TC : typingcontext_sound _ ?usrs _ ?uid , SS : syntactically_safe ?uid _ _ (Send _ _) _ |- _ ] =>
+          unfold typingcontext_sound in TC; split_ex; invert SS; process_ctx
+        end.
     
-    + eapply input_action_msg_queue in H45; eauto; split_ex; subst.
+    + process_actions.
       msg_queue_prop.
-      generalize (H39 _ _ _ H44 eq_refl); intro; split_ex; simpl in *.
-      eapply syntactically_safe_na in H7; eauto; split_ex.
-      assert (msg_pattern_safe (findUserKeys usrs') x0)
-        by (unfold typingcontext_sound in *; split_ex; invert H7; process_ctx; eauto).
       assert (msg_honestly_signed (findUserKeys usrs') cs0 msg0 = true) by eauto.
-      unfold msg_honestly_signed, msg_signing_key in H18;
+      unfold msg_honestly_signed, msg_signing_key in H17;
         destruct msg0;
         try discriminate;
         cases (cs0 $? c_id0);
         try discriminate;
         destruct c;
         eauto using action_matches_addnl_cipher_inp.
-    + eapply output_action_msg_queue in H45; eauto; split_ex; subst.
-      generalize (H39 _ _ _ H44 eq_refl); intro; split_ex; simpl in *.
-      eapply syntactically_safe_na in H7; eauto; split_ex.
-      unfold typingcontext_sound in *; split_ex; invert H7; process_ctx.
+    + process_actions.
       eauto using action_matches_addnl_cipher_out.
 
-  - destruct userData; simpl in *.
-    destruct ra.
+  - destruct userData; simpl in *; clean_map_lookups.
+    destruct ra; process_actions;
+      eauto using action_matches_addnl_cipher_inp , action_matches_addnl_cipher_out.
     
-    + eapply input_action_msg_queue in H43; eauto; split_ex; subst.
-      msg_queue_prop.
-      generalize (H37 _ _ _ H42 eq_refl); intro; split_ex; simpl in *.
-      eapply syntactically_safe_na in H5; eauto; split_ex.
-      assert (msg_pattern_safe (findUserKeys usrs') x0)
-        by (unfold typingcontext_sound in *; split_ex; invert H5; process_ctx; eauto).
-      assert (msg_honestly_signed (findUserKeys usrs') cs0 msg0 = true) by eauto.
-      unfold msg_honestly_signed, msg_signing_key in H16;
-        destruct msg0;
-        try discriminate;
-        cases (cs0 $? c_id0);
-        try discriminate;
-        destruct c;
-        eauto using action_matches_addnl_cipher_inp.
-    + eapply output_action_msg_queue in H43; eauto; split_ex; subst.
-      generalize (H37 _ _ _ H42 eq_refl); intro; split_ex; simpl in *.
-      eapply syntactically_safe_na in H5; eauto; split_ex.
-      unfold typingcontext_sound in *; split_ex; invert H5; process_ctx.
-      eauto using action_matches_addnl_cipher_out.
+    msg_queue_prop.
+    assert (MHS : msg_honestly_signed (findUserKeys usrs') cs0 msg0 = true) by eauto.
+    unfold msg_honestly_signed, msg_signing_key in MHS;
+      destruct msg0;
+      try discriminate;
+      cases (cs0 $? c_id0);
+      try discriminate;
+      destruct c;
+      eauto using action_matches_addnl_cipher_inp.
 
-  - destruct userData, ra; simpl in *.
+  - destruct userData; simpl in *; clean_map_lookups.
 
     Import ProtocolAutomation.
     Import SimulationAutomation.
 
-    + eapply input_action_msg_queue in H39; eauto; split_ex; subst.
-      msg_queue_prop.
-      generalize (H33 _ _ _ H38 eq_refl); intro; split_ex; simpl in *.
-      eapply syntactically_safe_na in H2; eauto; split_ex.
-      assert (msg_pattern_safe (findUserKeys usrs') x0)
-        by (unfold typingcontext_sound in *; split_ex; invert H2; process_ctx; eauto).
-      assert (msg_honestly_signed (findUserKeys usrs') cs' msg = true) by eauto.
+    destruct ra; process_actions.
 
-      unfold msg_honestly_signed, msg_signing_key in H13.
-      invert H8;
+    + msg_queue_prop.
+      assert (MHS : msg_honestly_signed (findUserKeys usrs') cs' msg = true) by eauto.
+      unfold msg_honestly_signed, msg_signing_key in MHS.
+
+      invert H6;
         clean_map_lookups;
         encrypted_ciphers_prop;
         eauto using message_content_eq_addnl_key_inv;
         keys_and_permissions_prop.
-
+      
       eapply InpEnc; eauto;
         repeat 
           match goal with
@@ -563,17 +528,12 @@ Proof.
             unfold not; intros GKS; eapply PHG in LK; split_ex; clean_map_lookups
           end.
 
-    + eapply output_action_msg_queue in H39; eauto; split_ex; subst.
-      generalize (H33 _ _ _ H38 eq_refl); intro; split_ex; simpl in *.
-      eapply syntactically_safe_na in H2; eauto; split_ex.
-      unfold typingcontext_sound in *; split_ex; invert H2; process_ctx.
-
-      invert H8;
+    + invert H6;
         clean_map_lookups;
         encrypted_ciphers_prop;
         eauto using message_content_eq_addnl_key_inv;
         keys_and_permissions_prop;
-        invert H14;
+        invert H13;
         clean_map_lookups.
 
       eapply OutSig; eauto;
@@ -600,25 +560,30 @@ Proof.
             unfold not; intros GKS; eapply PHG in LK; split_ex; clean_map_lookups
           end.
     
-  - destruct userData, ra; simpl in *.
+  - destruct userData; simpl in *; clean_map_lookups.
 
-    Import ProtocolAutomation.
-    Import SimulationAutomation.
+    destruct ra; process_actions.
 
-    + eapply input_action_msg_queue in H39; eauto; split_ex; subst.
-      msg_queue_prop.
-      generalize (H33 _ _ _ H38 eq_refl); intro; split_ex; simpl in *.
-      eapply syntactically_safe_na in H2; eauto; split_ex.
-      assert (msg_pattern_safe (findUserKeys usrs') x0)
-        by (unfold typingcontext_sound in *; split_ex; invert H2; process_ctx; eauto).
-      assert (msg_honestly_signed (findUserKeys usrs') cs' msg = true) by eauto.
+    + assert (MHS : msg_honestly_signed (findUserKeys usrs') cs' msg = true) by eauto.
 
-      unfold msg_honestly_signed, msg_signing_key in H13.
-      invert H8;
+      unfold msg_honestly_signed, msg_signing_key in MHS.
+      invert H6;
         clean_map_lookups;
         encrypted_ciphers_prop;
         eauto using message_content_eq_addnl_key_inv;
         keys_and_permissions_prop.
+      
+      eapply InpSig; eauto;
+        repeat 
+          match goal with
+          | [ |- content_eq _ _ _ ] =>
+            eapply message_content_eq_addnl_key_inv; eauto; intros
+          | [ H : (forall _ _, findKeysMessage ?msg $? _ = Some _ -> _), ARG : findKeysMessage ?msg $? _ = Some _ |- _ ] =>
+            eapply H in ARG; split_ex
+          | [ PHG : permission_heap_good ?gks ?honk, LK : ?honk $? ?k = Some _ |- ?gks $? ?k <> None ] =>
+            let GKS := fresh "GKS" in
+            unfold not; intros GKS; eapply PHG in LK; split_ex; clean_map_lookups
+          end.
 
       eapply InpEnc; eauto;
         repeat 
@@ -632,17 +597,12 @@ Proof.
             unfold not; intros GKS; eapply PHG in LK; split_ex; clean_map_lookups
           end.
 
-    + eapply output_action_msg_queue in H39; eauto; split_ex; subst.
-      generalize (H33 _ _ _ H38 eq_refl); intro; split_ex; simpl in *.
-      eapply syntactically_safe_na in H2; eauto; split_ex.
-      unfold typingcontext_sound in *; split_ex; invert H2; process_ctx.
-
-      invert H8;
+    + invert H6;
         clean_map_lookups;
         encrypted_ciphers_prop;
         eauto using message_content_eq_addnl_key_inv;
         keys_and_permissions_prop;
-        invert H14;
+        invert H13;
         clean_map_lookups.
 
       eapply OutSig; eauto;
@@ -671,47 +631,207 @@ Proof.
 Qed.
 
 Lemma no_model_step_other_user_silent_step :
-  forall t__hon t__adv uid uid' u u' U bd' lbl
+  forall t__hon t__adv uid uid' u U lbl
     (usrs : honest_users t__hon) (adv : user_data t__adv)  cs gks ks qmsgs mycs froms sents cur_n cmd iu,
     
     step_user Silent (Some uid) (build_data_step  U u) (usrs,adv,cs,gks,ks,qmsgs,mycs,froms,sents,cur_n,cmd)
     -> U.(users) $? uid = Some u
-    -> U.(users) $? uid' = Some u'
-    -> step_user lbl (Some uid') (build_data_step  U u') bd'
+    -> forall U', indexedRealStep uid' lbl U U'
+    (* -> U.(users) $? uid' = Some u' *)
+    (* -> step_user lbl (Some uid') (build_data_step  U u') bd' *)
     -> uid <> uid'
     -> goodness_predicates U
     -> syntactically_safe_U U
-    -> (forall st', model_step_user uid' (U, iu) st' -> False)
-    -> (forall st', model_step_user uid'
+    -> (forall st', indexedStep uid' (U, iu) st' -> False)
+    -> (forall st', indexedStep uid'
                   (mkUniverse (usrs $+ (uid, mkUserData ks cmd qmsgs mycs froms sents cur_n))
                               adv cs gks, iu)
                   st' -> False).
 
 Proof.
   unfold goodness_predicates; intros; split_ex.
-  generalize (H5 _ _ _ H0 eq_refl); intros; split_ex.
-  destruct u , u', U; simpl in *;
-    eapply no_model_step_other_user_silent_step' with (uid := uid) (uid' := uid'); try reflexivity; simpl; eauto; simpl.
+  invert H1.
+  generalize (H4 _ _ _ H0 eq_refl); intros; split_ex.
+  destruct u , U; simpl in *;
+    eapply no_model_step_other_user_silent_step' with (uid := uid) (uid' := uid');
+    try reflexivity; simpl; eauto; simpl.
 Qed.
 
 Notation "p1 @@ p2" := (IdealWorld.construct_permission p1 p2) (left associativity, at level 20).
 
 Section IdealWorldLemmas.
   Import IdealWorld.
+  Import IdealNotations.
+  Import ChMaps.
 
   Inductive perm_ge : permission -> permission -> Prop :=
   | Owner : forall p,
       perm_ge (true @@ true) p
-  | None : forall p,
+  | NoPerm : forall p,
       perm_ge p (false @@ false)
-  | Same : forall b1 b2,
+  | SamePerm : forall b1 b2,
       b1 <> b2
       -> perm_ge (b1 @@ b2) (b1 @@ b2)
   .
 
+  Notation "p1 @>@ p2" := (perm_ge p1 p2) (left associativity, at level 20).
+
+  Lemma perms_ge_refl :
+    forall p, p @>@ p.
+  Proof. intros; destruct p, read, write; econstructor; eauto; discriminate. Qed.
+
+  Hint Constructors perm_ge : core.
+  
+  Lemma perms_ge_trans :
+    forall p1 p2 p3, p1 @>@ p2 -> p2 @>@ p3 -> p1 @>@ p3.
+  Proof.
+    destruct p1 , read, write; intros; eauto;
+      repeat match goal with
+             | [ H : (?x @@ ?y) @>@ _ |- _ ] =>
+               is_not_var x; is_not_var y; invert H
+             end; eauto.
+  Qed.
+
+  Hint Resolve perms_ge_refl : core.
+
+  Definition chans_grown (chans chans' : channels) :=
+    (forall chid ch,
+        chans' #? chid = Some ch
+        -> chans #? chid = None
+        \/ chans #? chid = Some ch)
+  /\ (forall chid ch,
+        chans #? chid = Some ch
+        -> chans' #? chid = Some ch).
+
+  Definition user_perms_grown (ps ps' : permissions) :=
+    (forall pid p',
+        ps' $? pid = Some p'
+        -> ps $? pid = None
+        \/ exists p, ps $? pid = Some p /\ p' @>@ p)
+  /\ (forall pid p,
+        ps $? pid = Some p
+        -> ps' $? pid = Some p).
+
+  Lemma chans_grown_refl :
+    forall chans,
+      chans_grown chans chans.
+  Proof. unfold chans_grown; split; intros; eauto. Qed.
+
+  Lemma chans_grown_trans :
+    forall chans1 chans2 chans3,
+      chans_grown chans1 chans2
+      -> chans_grown chans2 chans3
+      -> chans_grown chans1 chans3.
+  Proof.
+    unfold chans_grown; intros; split_ex.
+    repeat simple apply conj; intros; eauto.
+    cases (chans1 #? chid); eauto.
+    eapply H2 in Heq.
+    eapply H1 in Heq.
+    rewrite Heq in H3; eauto.
+  Qed.
+    
+  Lemma user_perms_grown_refl :
+    forall ps,
+      user_perms_grown ps ps.
+  Proof. unfold user_perms_grown; split; intros; eauto. Qed.
+
+  Lemma user_perms_grown_trans :
+    forall ps1 ps2 ps3,
+      user_perms_grown ps1 ps2
+      -> user_perms_grown ps2 ps3
+      -> user_perms_grown ps1 ps3.
+  Proof.
+    unfold user_perms_grown; intros; split_ex.
+    repeat simple apply conj; intros; eauto.
+    eapply H0 in H3; split_ex.
+
+    cases (ps1 $? pid); eauto.
+    eapply H2 in Heq.
+    split_ors; clean_map_lookups.
+    right; eexists; split; eauto.
+  Qed.
+
+  Hint Resolve chans_grown_refl user_perms_grown_refl : core.
+
+  Lemma ideal_user_silent_step_chan_impact' :
+    forall A lbl bd bd',
+      @lstep_user A lbl bd bd'
+      -> forall chans chans' proto proto' ps ps',
+        bd = (chans, proto, ps)
+        -> bd' = (chans', proto', ps')
+        -> lbl = Silent
+        -> chans_grown chans chans'.
+  Proof.
+    induction 1; inversion 1; inversion 1; intros; subst; try discriminate; eauto.
+
+    unfold chans_grown; split; intros; eauto.
+    destruct (ChannelType.eq_dec (# ch_id) chid).
+    - invert e.
+      rewrite ChMap.P.F.add_eq_o in * by eauto; eauto.
+    - rewrite ChMap.P.F.add_neq_o in * by eauto; eauto.
+  Qed.
+
+  Lemma ideal_user_silent_step_perms_impact' :
+    forall A lbl bd bd',
+      @lstep_user A lbl bd bd'
+      -> forall chans chans' proto proto' ps ps',
+        bd = (chans, proto, ps)
+        -> bd' = (chans', proto', ps')
+        -> lbl = Silent
+        -> user_perms_grown ps ps'.
+  Proof.
+    induction 1; inversion 1; inversion 1; intros; subst; try discriminate; eauto.
+    unfold user_perms_grown; split; intros;
+      destruct (ch_id ==n pid); subst;
+        clean_map_lookups; eauto.
+  Qed.
+
+  Lemma ideal_universe_impact_silent_step :
+    forall A uid U U' u,
+      @indexedIdealStep A uid Silent U U'
+      -> U.(users) $? uid = Some u
+      -> chans_grown U.(channel_vector) U'.(channel_vector)
+      /\ (forall uid' u',
+            uid' <> uid
+            -> U.(users) $? uid' = Some u'
+            -> U'.(users) $? uid' = Some u')
+      /\ (exists u', U'.(users) $? uid = Some u'
+             /\ user_perms_grown u.(perms) u'.(perms)).
+  Proof.
+    intros * STEP USER; invert STEP; simpl;
+      repeat simple apply conj;
+      intros;
+      eauto using ideal_user_silent_step_chan_impact'.
+
+    clean_map_lookups; eexists; split; simpl; eauto using ideal_user_silent_step_perms_impact'.
+  Qed.
+
+  Lemma ideal_universe_impact_silent_steps :
+    forall A uid U U',
+      (@indexedIdealStep A uid Silent) ^* U U'
+      -> forall u, U.(users) $? uid = Some u
+      -> chans_grown U.(channel_vector) U'.(channel_vector)
+      /\ (forall uid' u',
+            uid' <> uid
+            -> U.(users) $? uid' = Some u'
+            -> U'.(users) $? uid' = Some u')
+      /\ (exists u', U'.(users) $? uid = Some u'
+             /\ user_perms_grown u.(perms) u'.(perms)).
+  Proof.
+    induction 1; intros; eauto.
+
+    generalize H; intros STEP; eapply ideal_universe_impact_silent_step in STEP; eauto; split_ex.
+    generalize H4; intros USR__y; eapply IHtrc in H4; split_ex.
+
+    repeat simple apply conj; intros;
+      eauto using chans_grown_trans , user_perms_grown_trans.
+  Qed.
+  
+    
 End IdealWorldLemmas.
 
-Lemma no_model_step_other_user_labeled_step :
+Lemma no_model_step_other_user_labeled_step' :
   forall t t__hon t__adv suid lbl bd bd',
 
     step_user lbl suid bd bd'
@@ -725,128 +845,115 @@ Lemma no_model_step_other_user_labeled_step :
       -> suid = Some uid
       -> lbl = Action ra
       -> forall cmdc, usrs $? uid = Some (mkUserData ks cmdc qmsgs mycs froms sents n)
-      -> forall ud', usrs $? uid' = Some ud'
-      -> forall lbl' bd'', step_user lbl' (Some uid') (build_data_step (mkUniverse usrs adv cs gks) ud') bd''
+      -> forall lbl' ru', indexedRealStep uid' lbl' (mkUniverse usrs adv cs gks) ru'
+      (* -> forall ud', usrs $? uid' = Some ud' *)
+      (* -> forall lbl' bd'', step_user lbl' (Some uid') (build_data_step (mkUniverse usrs adv cs gks) ud') bd'' *)
       (* arguments to fill out label alignment for uid step above *)                                  
-      -> (istepSilent) ^* iu iu'
-      -> IdealWorld.lstep_universe iu' (Action ia) iu''
+      -> (indexedIdealStep uid Silent) ^* iu iu'    
+      -> indexedIdealStep uid (Action ia) iu' iu''
       -> action_matches cs gks ra ia
       -> uid <> uid'
-      -> forall cmdc,
-        (forall st', model_step_user
+      -> forall cmdc',
+        (forall st', indexedStep
                   uid' 
                   (mkUniverse usrs adv cs gks, iu)
                   st' -> False)
-      -> (forall st', model_step_user
+      -> (forall st', indexedStep
                   uid'
-                  (mkUniverse (usrs' $+ (uid, mkUserData ks' cmdc qmsgs' mycs' froms' sents' n'))
+                  (mkUniverse (usrs' $+ (uid, mkUserData ks' cmdc' qmsgs' mycs' froms' sents' n'))
                               adv' cs' gks', iu'')
                   st' -> False).
 Proof.
-
   intros * STEP;
     generalize STEP;
     induction 1; inversion 1; inversion 1;
       intros; subst; eauto; clean_context.
 
-  - solve_model_step_block STEP.
+  - repeat
+      match goal with
+      | [ H : indexedStep _ _ _ |- _ ] => invert H
+      | [ H : indexedRealStep _ _ _ _ |- _ ] => invert H
+      end; simpl in *; clean_map_lookups.
 
-    invert H8.
-    + econstructor 1; eauto.
-      assert (ia = IdealWorld.Input m__iw ch_id cs1 ps) by admit; eauto.
-      admit.
-
-      invert H13; [ econstructor 1 | econstructor 2 ]; simpl in *; eauto;
-        intros;
-        autorewrite with find_user_keys in *; eauto;
-          specialize (H15 u); destruct (u ==n uid); subst; clean_map_lookups; eauto 8.
-
-      (* including message heap keys helps here 
-       * still worried aobut progression of ideal world, though
-       *)
-      admit.
-      admit.
-      admit.
-      admit.
-
-    + econstructor 2; eauto.
-      assert (ia = IdealWorld.Output m__iw ch_id cs1 ps) by admit; eauto.
-
-      invert H12; [ econstructor 1 | econstructor 2 ]; simpl in *; eauto;
-        intros;
-        autorewrite with find_user_keys in *; eauto;
-          specialize (H14 u); destruct (u ==n uid); subst; clean_map_lookups; eauto 8.
-
-      (* including message heap keys helps here 
-       * still worried aobut progression of ideal world, though
-       *)
-      admit.
-      admit.
-      admit.
-      admit.
-
-  - destruct (rec_u_id ==n uid'); subst; clean_map_lookups;
-      solve_model_step_block STEP; simpl in *.
-
-    + dt bd'';
-        destruct ud';
-        simpl in *.
-
-      assert (lbl' = Silent) by 
+    + assert (lbl' = Silent) by
           (clean_map_lookups;
            eapply (user_step_label_deterministic' _ _ _ _ _ _ _ STEP);
            eauto; unfold build_data_step; simpl; eauto); subst.
-      
-      eapply H40; econstructor 1; unfold build_data_step, buildUniverse; simpl; eauto; simpl.
+      eapply H39.
+      econstructor 1; eauto.
 
-    + dt bd'';
-        destruct ud';
-        simpl in *.
-
-      assert (lbl' = Action ra) by 
-          (clean_map_lookups;
-           eapply (user_step_label_deterministic' _ _ _ _ _ _ _ STEP);
-           eauto; unfold build_data_step; simpl; eauto); subst.
-      
-      eapply H40; econstructor 2; unfold build_data_step, buildUniverse; simpl; eauto; simpl.
-
-      invert H11.
-      * econstructor 1; eauto.
-        assert (ia = IdealWorld.Input m__iw ch_id cs1 ps) by admit; eauto.
-        admit.
-        
-        invert H16; [ econstructor 1 | econstructor 2 ]; simpl in *; eauto;
-          intros;
-          autorewrite with find_user_keys in *; eauto;
-            specialize (H18 u); destruct (u ==n uid); subst; clean_map_lookups; eauto 8.
-
-        all: admit.
-
-      * admit.
-
-    + dt bd'';
-        destruct userData;
-        simpl in *.
-
-      assert (lbl' = Silent) by
-          ( clean_map_lookups;
-            eapply (user_step_label_deterministic' _ _ _ _ _ _ _ STEP) with (uid' := uid');
-            eauto; unfold build_data_step; simpl; eauto); subst.
-      
-      eapply H40; econstructor 1; unfold build_data_step, buildUniverse; simpl; eauto; simpl.
-
-    + dt bd'';
-        destruct userData;
-        simpl in *.
-
+    + destruct userData0; simpl in *.
       assert (lbl' = Action ra) by
-          ( clean_map_lookups;
-            eapply (user_step_label_deterministic' _ _ _ _ _ _ _ STEP) with (uid' := uid');
-            eauto; unfold build_data_step; simpl; eauto); subst.
+          (clean_map_lookups;
+           eapply (user_step_label_deterministic' _ _ _ _ _ _ _ STEP);
+           eauto; unfold build_data_step; simpl; eauto); subst.
+      unfold build_data_step in *; simpl in *.
+      eapply H39; clear H39; econstructor 2; simpl.
+      econstructor.
+      eassumption.
+      eassumption.
+      reflexivity.
+      admit.
+      admit.
+      admit.
 
-      eapply H40; econstructor 2; unfold build_data_step, buildUniverse; simpl; eauto; simpl.
+  - repeat
+      match goal with
+      | [ H : indexedStep _ _ _ |- _ ] => invert H
+      | [ H : indexedRealStep _ _ _ _ |- _ ] => invert H
+      end; simpl in *; clean_map_lookups.
+
+    + assert (lbl' = Silent).
+      destruct (rec_u_id ==n uid'); subst; clean_map_lookups.
+      eapply (user_step_label_deterministic' _ _ _ _ _ _ _ STEP) with (uid'0 := uid');
+        eauto; unfold build_data_step; simpl; eauto.
+      eapply (user_step_label_deterministic' _ _ _ _ _ _ _ STEP) with (uid' := uid');
+        eauto; unfold build_data_step; simpl; eauto.
+      subst.
+      eapply H39.
+      econstructor 1; eauto.
+
+    + destruct userData0; simpl in *.
+      assert (lbl' = Action ra).
+      destruct (rec_u_id ==n uid'); subst; clean_map_lookups.
+      eapply (user_step_label_deterministic' _ _ _ _ _ _ _ STEP) with (uid'0 := uid');
+        eauto; unfold build_data_step; simpl; eauto.
+      eapply (user_step_label_deterministic' _ _ _ _ _ _ _ STEP) with (uid' := uid');
+        eauto; unfold build_data_step; simpl; eauto.
+      subst.
+      eapply H39; clear H39; econstructor 2; simpl.
+      econstructor.
+      eassumption.
+      eassumption.
+      reflexivity.
+    
       
 Admitted.
+
+Lemma no_model_step_other_user_labeled_step :
+  forall t__hon t__adv uid uid' u U lbl ra
+    (usrs : honest_users t__hon) (adv : user_data t__adv) cs gks ks qmsgs mycs froms sents cur_n cmd iu,
+    
+    step_user (Action ra) (Some uid) (build_data_step  U u) (usrs,adv,cs,gks,ks,qmsgs,mycs,froms,sents,cur_n,cmd)
+    -> U.(users) $? uid = Some u
+    -> forall U', indexedRealStep uid' lbl U U'
+    -> forall iu' iu'' ia, (indexedIdealStep uid Silent) ^* iu iu'    
+    -> indexedIdealStep uid (Action ia) iu' iu''
+    -> action_matches U.(all_ciphers) U.(all_keys) ra ia
+    (* -> U.(users) $? uid' = Some u' *)
+    (* -> step_user lbl (Some uid') (build_data_step  U u') bd' *)
+    -> uid <> uid'
+    -> goodness_predicates U
+    -> syntactically_safe_U U
+    -> (forall st', indexedStep uid' (U, iu) st' -> False)
+    -> (forall st', indexedStep uid'
+                  (mkUniverse (usrs $+ (uid, mkUserData ks cmd qmsgs mycs froms sents cur_n))
+                              adv cs gks, iu'')
+                  st' -> False).
+Proof.
+  intros; destruct U, u; unfold build_data_step in *; simpl in *.
+  eapply no_model_step_other_user_labeled_step'; eauto.
+Qed.
 
 Lemma stuck_model_violation_step' :
   forall t__hon t__adv st st' b,
@@ -854,10 +961,10 @@ Lemma stuck_model_violation_step' :
     -> lameAdv b (fst st).(adversary)
     -> goodness_predicates (fst st)
     -> syntactically_safe_U (fst st)
-    -> stuck_model_step_user_stuck_user st'
-    -> stuck_model_step_user_stuck_user st.
+    -> not_stuck_by_labels st'
+    -> not_stuck_by_labels st.
 Proof.
-  unfold stuck_model_step_user_stuck_user; intros.
+  unfold not_stuck_by_labels; intros.
 
   invert H; simpl in *.
 
@@ -877,64 +984,67 @@ Proof.
       rewrite add_neq_o in H3 by auto.
       specialize (H3 _ H7); simpl in H3.
 
-      generalize (no_model_step_other_user_silent_step _ _ _ _ _ _ _ _ _ _ _ _ _ _ _ _ _ _ _ _ _ H8 H H4 H6 n H1 H2 H5);
+      generalize (no_model_step_other_user_silent_step _ _ _ _ _ _ _ _ _ _ _ _ _ _ _ _ _ _ _
+                                                       H8 H _ H6 n H1 H2 H5);
         intros NOMODEL.
+
+      generalize H6; invert H6; simpl in *; intros; clean_map_lookups.
 
       assert (OU : usrs $+ (u_id, mkUserData ks cmd qmsgs mycs froms sents cur_n) $? uid =
                    Some (mkUserData key_heap protocol (msg_heap ++ x) c_heap from_nons sent_nons cur_nonce))
         by (clean_map_lookups; trivial).
 
-      generalize (step_reorder_simple _ _ _ _ _ _ _ _ _ _ _ _ _ _ _ _ _ _ _ _ _ H8 H H4 H6 n _ _ eq_refl OU);
+      generalize (step_reorder_simple _ _ _ _ _ _ _ _ _ _ _ _ _ _ _ _ _ _ _ _ _ H8 H H4 H10 n _ _ eq_refl OU);
         intros;
         split_ex.
 
-      eapply H3 in NOMODEL; try contradiction; eauto.
+      dt x0; eapply H3 in NOMODEL; eauto.
 
   (* labeled case -- this will perhaps be a bit more difficult because of the ideal world *)
-  - invert H7.
-    simpl in *.
-    (* unfold buildUniverse, build_data_step in *; simpl in *. *)
-
-    destruct (u_id ==n uid); subst; clean_map_lookups.
+  - destruct (uid0 ==n uid); subst; clean_map_lookups.
     + eapply H5.
       econstructor 2; eauto.
-    + generalize H9; intros OUSTEP.
+    + generalize H7; intros OUSTEP; invert OUSTEP.
 
-      destruct ru, u; simpl in *.
-      eapply impact_from_other_user_step in OUSTEP; eauto; split_ex.
+      destruct ru, u, userData; simpl in *.
+      generalize H11; intros.
+      unfold build_data_step in H11; simpl in *.
+      eapply impact_from_other_user_step with (u_id2 := uid) in H11; eauto; split_ex.
 
-      specialize (H1 uid).
-      rewrite add_neq_o in H1 by auto.
-      specialize (H1 _ H5); simpl in H1.
+      specialize (H3 uid).
+      rewrite add_neq_o in H3 by auto.
+      specialize (H3 _ H11); simpl in H3.
 
-      destruct userData; simpl in *.
-      pose proof (no_model_step_other_user_labeled_step
-                    _ _ _ _ _ _ _ H9
-                    _ _ _ _ _ _ _ _ _ _ _ _ _ _ _ _ _ _ _ _ _ _ _ _ ra ia iu iu' iu''
-                    eq_refl eq_refl eq_refl eq_refl _ H _ H2 _ _ H4 H6 H7 H8 n cmd H3) as NOMODEL.
-      specialize (H1 NOMODEL).
+      generalize (no_model_step_other_user_labeled_step _ _ _ _ _ _ _ _ _ _ _ _ _ _ _ _ _ _ _ _
+                                                        H12 H _ H6 _ _ _ H8 H9 H10 n
+                                                        H1 H2 H5);
+        intros NOMODEL.
 
-      dt bd.
-      pose proof (step_reorder _ _ _ _ _ _ _ _ H9 eq_refl _ _ _ _ _ _ H4 eq_refl) as REORDER.
-      generalize H; intros USR; eapply REORDER in USR; eauto; clear REORDER.
-      split_ex.
-      unfold build_data_step in H7; simpl in H7.
-      eapply H1; eauto.
+      invert H6; simpl in *.
+      clean_map_lookups.
+      assert (OU : usrs $+ (uid0, mkUserData ks cmd qmsgs mycs froms sents cur_n) $? uid =
+                   Some (mkUserData key_heap protocol (msg_heap ++ x) c_heap from_nons sent_nons cur_nonce))
+        by (clean_map_lookups; trivial).
 
-Admitted.
+      pose proof (step_reorder_simple _ _ _ _ _ _ _ _ _ _ _ _ _ _ _ _ _ _ _ _ _ H12 H H4 H14 n _ _ eq_refl OU);
+        intros;
+        split_ex.
+
+      dt x0; eapply H3 in NOMODEL; eauto.
+Qed.
 
 Lemma stuck_model_violation_step :
   forall t__hon t__adv st st' b,
     @step t__hon t__adv st st'
     -> lameAdv b (fst st).(adversary)
-    -> ~ stuck_model_step_user_stuck_user st
-    -> ~ stuck_model_step_user_stuck_user st'.
+    -> goodness_predicates (fst st)
+    -> syntactically_safe_U (fst st)
+    -> ~ not_stuck_by_labels st
+    -> ~ not_stuck_by_labels st'.
 Proof.
   unfold not; intros.
   eauto using stuck_model_violation_step'.
 Qed.
-
-    
 
 
 
@@ -947,7 +1057,7 @@ Module Type SyntacticallySafeProtocol.
   Parameter iu0 : IdealWorld.universe t__hon.
   Parameter ru0 : RealWorld.universe t__hon t__adv.
 
-  Notation SYS := (S ru0 iu0).
+  Notation SYS := (TrS ru0 iu0).
 
   Axiom U_good : universe_starts_sane b ru0.
   Axiom universe_starts_safe : universe_ok ru0 /\ adv_universe_ok ru0 /\ syntactically_safe_U ru0.
@@ -955,7 +1065,7 @@ Module Type SyntacticallySafeProtocol.
   Axiom safe_invariant : invariantFor
                            SYS
                            (fun st => no_resends_U (fst st)
-                                 /\ stuck_model_step_user_stuck_user st ).
+                                 /\ not_stuck_by_labels st ).
 
 End SyntacticallySafeProtocol.
 
@@ -965,7 +1075,7 @@ Module ProtocolSimulates (Proto : SyntacticallySafeProtocol).
   Lemma no_resends_inv : invariantFor SYS (fun st => no_resends_U (fst st)).
   Proof. eapply invariant_weaken; [ apply safe_invariant | firstorder idtac ]. Qed.
 
-  Lemma stuck_not_misaligned_inv : invariantFor SYS stuck_model_step_user_stuck_user.
+  Lemma stuck_not_misaligned_inv : invariantFor SYS not_stuck_by_labels.
   Proof. eapply invariant_weaken; [ apply safe_invariant | firstorder eauto ]. Qed.
 
   Hint Resolve no_resends_inv stuck_not_misaligned_inv.
@@ -1172,6 +1282,35 @@ Module ProtocolSimulates (Proto : SyntacticallySafeProtocol).
     unfold buildUniverse, peel_adv; simpl; trivial.
   Qed.
 
+  Lemma reachable_from_labeled_step' :
+    forall iu (ru U U' : RealWorld.universe t__hon t__adv) a__r,
+      SYS.(Step) ^* (ru0,iu0) (ru,iu)
+      -> forall uid, indexedRealStep uid (Action a__r) U U'
+
+      -> lameAdv b U.(adversary)
+      -> ru.(users) = U.(users)
+      -> ru.(all_ciphers) = U.(all_ciphers)
+      -> ru.(all_keys) = U.(all_keys)
+      -> exists U'',
+          indexedRealStep uid (Action a__r) ru U''
+          (* step_universe ru (Action a__r) U'' *)
+          /\ peel_adv U' = peel_adv U''.
+  Proof.
+    intros.
+    assert (lameAdv b ru.(adversary))
+      by (pose proof U_good; unfold universe_starts_sane, adversary_is_lame in *; split_ands; eauto with safe).
+    
+    destruct ru; destruct U; simpl in *; subst.
+    invert H0.
+
+    destruct userData; unfold build_data_step in *; simpl in *.
+
+    eapply lame_adv_no_impact_labeled_step in H3; split_ex.
+    eexists; split.
+    econstructor; unfold build_data_step; eauto; simpl in *.
+    unfold buildUniverse, peel_adv; simpl; trivial.
+  Qed.
+
   Lemma simsilent : simulates_silent_step (lameAdv b) R.
   Proof.
     hnf
@@ -1193,35 +1332,35 @@ Module ProtocolSimulates (Proto : SyntacticallySafeProtocol).
     
   Qed.
 
-  Lemma message_eq_adv_change :
-    forall {t t1 t2} (m__rw : crypto t) (m__iw : IdealWorld.message.message t)
-      (U U' : RealWorld.universe t1 t2) (U__i : IdealWorld.universe t1) ch_id,
-      message_eq m__rw U m__iw U__i ch_id
-      -> users U = users U'
-      -> all_ciphers U = all_ciphers U'
-      -> all_keys U = all_keys U'
-      -> message_eq m__rw U' m__iw U__i ch_id.
-  Proof.
-    intros * MEQ RWU RWC RWK.
-    invert MEQ; [ econstructor 1 | econstructor 2 ]
-    ; rewrite <- ?RWU, <- ?RWC, <- ?RWK
-    ; eauto.
-  Qed.
+  (* Lemma message_eq_adv_change : *)
+  (*   forall {t t1 t2} (m__rw : crypto t) (m__iw : IdealWorld.message.message t) *)
+  (*     (U U' : RealWorld.universe t1 t2) (U__i : IdealWorld.universe t1) ch_id, *)
+  (*     message_eq m__rw U m__iw U__i ch_id *)
+  (*     -> users U = users U' *)
+  (*     -> all_ciphers U = all_ciphers U' *)
+  (*     -> all_keys U = all_keys U' *)
+  (*     -> message_eq m__rw U' m__iw U__i ch_id. *)
+  (* Proof. *)
+  (*   intros * MEQ RWU RWC RWK. *)
+  (*   invert MEQ; [ econstructor 1 | econstructor 2 ] *)
+  (*   ; rewrite <- ?RWU, <- ?RWC, <- ?RWK *)
+  (*   ; eauto. *)
+  (* Qed. *)
 
-  Hint Resolve message_eq_adv_change : safe.
+  (* Hint Resolve message_eq_adv_change : safe. *)
   Hint Constructors action_matches : safe.
   
-  Lemma action_matches_adv_change :
-    forall {t1 t2} (U U' : RealWorld.universe t1 t2) (U__i : IdealWorld.universe t1) a__r a__i,
-      action_matches a__r U a__i U__i
-      -> users U = users U'
-      -> all_ciphers U = all_ciphers U'
-      -> all_keys U = all_keys U'
-      -> action_matches a__r U' a__i U__i.
-  Proof.
-    intros * AM RWU RWC RWK.
-    invert AM; eauto with safe.
-  Qed.
+  (* Lemma action_matches_adv_change : *)
+  (*   forall {t1 t2} (U U' : RealWorld.universe t1 t2) (U__i : IdealWorld.universe t1) a__r a__i, *)
+  (*     action_matches a__r U a__i U__i *)
+  (*     -> users U = users U' *)
+  (*     -> all_ciphers U = all_ciphers U' *)
+  (*     -> all_keys U = all_keys U' *)
+  (*     -> action_matches a__r U' a__i U__i. *)
+  (* Proof. *)
+  (*   intros * AM RWU RWC RWK. *)
+  (*   invert AM; eauto with safe. *)
+  (* Qed. *)
 
   Lemma simlabeled : simulates_labeled_step (lameAdv b) R.
   Proof.
@@ -1229,27 +1368,31 @@ Module ProtocolSimulates (Proto : SyntacticallySafeProtocol).
     ; intros * REL UOK AUOK LAME * STEP
     ; invert REL.
 
-    generalize (reachable_from_labeled_step _ _ _ _ _ H3 STEP LAME H H1 H2);
+    pose proof ( indexedRealStep_real_step STEP ) as STEPU.
+
+    generalize (reachable_from_labeled_step' _ _ _ _ _ H3 _ STEP LAME H H1 H2);
       intros; split_ex.
 
     pose proof stuck_not_misaligned_inv.
     unfold invariantFor, SYS in H5; simpl in H5.
     assert ( (ru0,iu0) = (ru0,iu0) \/ False ) as ARG by eauto.
     specialize (H5 _ ARG _ H3).
-    apply stuck_model_step_user_stuck_user_implies_labels_align in H5.
+    apply not_stuck_by_labels_implies_labels_align in H5.
 
-    specialize (H5 _ _ H0); split_ex; rewrite H4; (do 3 eexists);
+    (* assert (indexedRealStep uid (Action ra) ru U__r'). *)
+    (* destruct ru, U__r; simpl in *; subst; simpl in *. *)
+    (* invert STEP; simpl in *; clean_map_lookups; econstructor; eauto. *)
+
+    specialize (H5 _ _ _ H0); split_ex; rewrite H4; (do 3 eexists);
       repeat simple apply conj; eauto.
 
-    - invert H7; eauto with safe.
-      
-    - econstructor.
+    econstructor.
 
-      eapply trcEnd_trc.
-      generalize (trc_trcEnd H3); intros.
-      econstructor; eauto.
-      unfold SYS; simpl.
-      econstructor; eauto.
+    eapply trcEnd_trc.
+    generalize (trc_trcEnd H3); intros.
+    econstructor; eauto.
+    unfold SYS; simpl.
+    econstructor; eauto.
   Qed.
 
   Lemma ss_implies_next_safe :
@@ -1382,17 +1525,18 @@ Module ProtocolSimulates (Proto : SyntacticallySafeProtocol).
       apply H10 in H; split_ex; subst; eauto.
   Qed.
 
-  Lemma model_step_implies_step :
+  Lemma indexedStep_implies_step :
     forall t__hon t__adv uid st st',
-      @model_step_user t__hon t__adv uid st st'
+      @indexedStep t__hon t__adv uid st st'
       -> step st st'.
   Proof.
-    intros * MS.
-    invert MS; intros.
-    - econstructor 1.
-      econstructor; eauto.
-    - econstructor 2; eauto.
-      econstructor; eauto.
+    intros;
+      repeat
+        match goal with
+        | [ H : indexedStep _ _ _ |- _ ] => invert H
+        | [ H : indexedRealStep _ _ _ _ |- _ ] => invert H
+        end;
+      [ econstructor 1 | econstructor 2 ]; eauto.
   Qed.
 
   Lemma step_na_recur :
@@ -1417,7 +1561,7 @@ Module ProtocolSimulates (Proto : SyntacticallySafeProtocol).
     eapply IHnextAction in H0; eauto. split_ex.
     simpl.
 
-    Set Printing Implicit.
+    (* Set Printing Implicit. *)
     
     dt x; eexists; eapply StepBindRecur; eauto.
 
@@ -1457,10 +1601,10 @@ Module ProtocolSimulates (Proto : SyntacticallySafeProtocol).
     rename U__i into iu.
     red. intros.
 
-    destruct (classic (exists st', model_step_user u_id (ru,iu) st')).
+    destruct (classic (exists st', indexedStep u_id (ru,iu) st')).
     - split_ex.
       rename x1 into st'.
-      pose proof (model_step_implies_step _ _ _ _ _ H11) as STEP.
+      pose proof (indexedStep_implies_step _ _ _ _ _ H11) as STEP.
       assert (STEPS' : (@step t__hon t__adv) ^* (ru,iu) st') by (eauto using TrcFront).
       pose proof (trc_trans H3 STEPS') as STEPS.
 
@@ -1474,6 +1618,9 @@ Module ProtocolSimulates (Proto : SyntacticallySafeProtocol).
       rewrite Forall_natmap_forall in H0.
       
       destruct ru; invert H11;
+        match goal with
+        | [ H : indexedRealStep _ _ _ _ |- _] => invert H
+        end;
         unfold build_data_step in *;
         clean_map_lookups;
         simpl in *;
@@ -1492,7 +1639,7 @@ Module ProtocolSimulates (Proto : SyntacticallySafeProtocol).
       + eapply nextAction_couldBe in H10; eauto.
       + apply H16 in H14; split_ex; subst; eauto.
       + exfalso.
-        assert (forall st', model_step_user u_id (ru,iu) st' -> False) by eauto using not_ex_all_not.
+        assert (forall st', indexedStep u_id (ru,iu) st' -> False) by eauto using not_ex_all_not.
         pose proof stuck_not_misaligned_inv as NOTMISAL.
         specialize (NOTMISAL _ ARG _ H3).
         eapply NOTMISAL in H14.
@@ -1514,11 +1661,14 @@ Module ProtocolSimulates (Proto : SyntacticallySafeProtocol).
         
         split_ex.
 
-        assert (forall st', model_step_user u_id (ru,iu) st' -> False) by eauto using not_ex_all_not.
+        assert (forall st', indexedStep u_id (ru,iu) st' -> False) by eauto using not_ex_all_not.
         eapply NOTMISAL in H20; eauto.
         unfold build_data_step in H20; simpl in H20; eauto.
 
-        dt x5; eapply step_na_recur in H10; eauto; split_ex; eauto.
+        dt x5; eapply step_na_recur in H10; eauto.
+        split_ex; eauto.
+        dt x5.
+        eapply H20; econstructor; eauto.
   Qed.
 
   Hint Resolve simsilent simlabeled simsafe : safe.
